src/ssa/ndopsem_dsop.v
@@ -1,0 +1,1173 @@
+Add LoadPath "./ott".
+Add LoadPath "./monads".
+Add LoadPath "./compcert".
+Add LoadPath "../../../theory/metatheory_8.3".
+Require Import ssa_def.
+Require Import ssa_lib.
+Require Import List.
+Require Import Arith.
+Require Import tactics.
+Require Import monad.
+Require Import trace.
+Require Import Metatheory.
+Require Import genericvalues.
+Require Import alist.
+Require Import Values.
+Require Import Memory.
+Require Import Integers.
+Require Import Coqlib.
+Require Import targetdata.
+Require Import Ensembles.
+Require Import ssa_dynamic.
+Require Import Floats.
+Require Import ndopsem.
+
+Export NDopsem.
+Export LLVMopsem.
+
+Definition instantiate_gv (gv:GenericValue) (gvs:GVs) : Prop :=
+match gv with
+| (Vundef, _)::nil => Inhabited _ gvs
+| _ => Same_set _ (Singleton GenericValue gv) gvs
+end.
+
+Fixpoint instantiate_locals (lc1 : GVMap) (lc2 : GVsMap) : Prop :=
+match lc1, lc2 with
+| nil, nil => True
+| (id1,gv1)::lc1', (id2,gvs2)::lc2' => 
+    id1=id2 /\ instantiate_gv gv1 gvs2 /\ instantiate_locals lc1' lc2'
+| _, _ => False
+end.
+
+Definition instantiate_EC (ec1 : LLVMopsem.ExecutionContext) 
+  (ec2 : NDopsem.ExecutionContext) : Prop :=
+match ec1, ec2 with
+| LLVMopsem.mkEC f1 b1 cs1 tmn1 lc1 als1, NDopsem.mkEC f2 b2 cs2 tmn2 lc2 als2 =>
+    f1 = f2 /\ b1 = b2 /\ cs1 = cs2 /\ tmn1 = tmn2 /\
+    instantiate_locals lc1 lc2 /\ als1 = als2
+end.
+
+Fixpoint instantiate_ECs (ecs1 : LLVMopsem.ECStack) (ecs2 : NDopsem.ECStack) 
+  : Prop :=
+match ecs1, ecs2 with
+| nil, nil => True
+| ec1::ecs1', ec2::ecs2' => instantiate_EC ec1 ec2 /\ instantiate_ECs ecs1' ecs2'
+| _, _ => False
+end.
+
+Definition instantiate_State (st1 : LLVMopsem.State) (st2 : NDopsem.State) 
+  : Prop :=
+match st1, st2 with
+| LLVMopsem.mkState s1 td1 ps1 ecs1 gl1 fs1 M1,
+  NDopsem.mkState s2 td2 ps2 ecs2 gl2 fs2 M2 =>
+    s1 = s2 /\ td1 = td2 /\ ps1 = ps2 /\ instantiate_ECs ecs1 ecs2 /\ gl1 = gl2
+    /\ fs1 = fs2 /\ M1 = M2
+end.
+
+Ltac simpl_nd_llvmds :=
+  match goal with
+  | [Hsim : instantiate_State {| ECS := _::_::_ |} ?st2 |- _ ] =>
+     destruct st2 as [S' TD' Ps' ECs' gl' fs' M'];
+     destruct Hsim as [eq1 [eq2 [eq3 [Hsim [eq4 [eq5 eq6]]]]]]; subst;
+     destruct ECs' as [|[f1' b1' cs1' tmn1' lc1' als1'] ECs']; 
+       try solve [inversion Hsim];
+     simpl in Hsim; destruct Hsim as [Hsim1 Hsim2];
+     destruct ECs' as [|[f2' b2' cs2' tmn2' lc2' als2'] ECs'];
+       try solve [inversion Hsim2];
+     destruct Hsim2 as [Hsim2 Hsim3];
+     destruct Hsim1 as [J1 [J2 [J3 [J4 [Hsim1 J6]]]]]; subst;
+     destruct Hsim2 as [J1 [J2 [J3 [J4 [Hsim2 J6]]]]]; subst
+  | [Hsim : instantiate_State {| ECS := _::_|} ?st2 |- _ ] =>
+     destruct st2 as [S' TD' Ps' ECs' gl' fs' M'];
+     destruct Hsim as [eq1 [eq2 [eq3 [Hsim [eq4 [eq5 eq6]]]]]]; subst;
+     destruct ECs' as [|[f1' b1' cs1' tmn1' lc1' als1'] ECs']; 
+       try solve [inversion Hsim];
+     simpl in Hsim; destruct Hsim as [Hsim1 Hsim2];
+     destruct Hsim1 as [J1 [J2 [J3 [J4 [Hsim1 J6]]]]]; subst
+  end.
+
+Lemma instantiate_locals__lookup : forall lc1 lc2 id1 gv1,
+  instantiate_locals lc1 lc2 -> 
+  lookupAL _ lc1 id1 = Some gv1 ->
+  exists gvs2, lookupAL _ lc2 id1 = Some gvs2 /\ instantiate_gv gv1 gvs2.
+Proof.
+  induction lc1; destruct lc2; simpl; intros id1 gv1 Hinst Hlk.  
+    inv Hlk.
+    inv Hinst.
+    destruct a. inv Hinst.     
+
+    destruct a. destruct p.
+    destruct Hinst as [J1 [J2 J3]]; subst.
+    destruct (id1 == i1); subst; eauto.
+      inv Hlk. eauto.
+Qed.
+
+Lemma same_singleton_set : forall gv,
+  Same_set GenericValue (Singleton _ gv) (Singleton _ gv).
+Proof.
+  unfold Same_set, Included. auto.
+Qed.
+
+Lemma instantiate_gv__gv2gvs : forall gv, instantiate_gv gv ($ gv $).
+Proof.
+  intros.
+  assert (J:=@gv2gvs__inhabited gv).
+  destruct gv; simpl; auto using same_singleton_set.
+    destruct p; simpl.
+    destruct v; simpl; auto using same_singleton_set.     
+    destruct gv; simpl; auto using same_singleton_set.     
+Qed.
+
+Lemma instantiate_locals__getOperandValue : forall TD v lc1 lc2 gl gv1,
+  instantiate_locals lc1 lc2 -> 
+  getOperandValue TD v lc1 gl = Some gv1 ->
+  exists gvs2, NDopsem.getOperandValue TD v lc2 gl = Some gvs2 /\
+    instantiate_gv gv1 gvs2.
+Proof.
+  intros.
+  destruct v; simpl in *.
+    eapply instantiate_locals__lookup; eauto.
+    exists ($ gv1 $). unfold mmap. rewrite H0. simpl. 
+    auto using instantiate_gv__gv2gvs.
+Qed.
+
+Ltac tinv H := try solve [inv H].
+
+Lemma instantiate_locals__updateAddAL : forall gv3 gvs3',
+  instantiate_gv gv3 gvs3' ->
+  forall lc1 lc2 id0,
+  instantiate_locals lc1 lc2 -> 
+  instantiate_locals (updateAddAL GenericValue lc1 id0 gv3)
+    (updateAddAL GVs lc2 id0 gvs3').
+Proof.
+  induction lc1; destruct lc2; simpl; intros id0 H1; auto.
+    inv H1.  
+    destruct a. inv H1.
+    destruct a. destruct p. destruct H1 as [eq [H1 H2]]; subst.
+    destruct (id0 == i1); subst; simpl.
+      split; auto.
+      split; auto.
+Qed.   
+
+Lemma instantiate_locals__returnUpdateLocals : forall TD lc1 lc2 lc1' lc2' Result
+    gl lc1'' c,
+  instantiate_locals lc1 lc2 -> 
+  instantiate_locals lc1' lc2' -> 
+  returnUpdateLocals TD c Result lc1 lc1' gl = ret lc1'' ->
+  exists lc2'', 
+    NDopsem.returnUpdateLocals TD c Result lc2 lc2' gl = ret lc2'' /\
+    instantiate_locals lc1'' lc2''. 
+Proof.
+  intros.
+  unfold returnUpdateLocals in H1.
+  remember (getOperandValue TD Result lc1 gl) as R.
+  destruct R; tinv H1.
+  symmetry in HeqR.
+  eapply instantiate_locals__getOperandValue in HeqR; eauto.
+  destruct HeqR as [gvs2 [J1 J2]].
+  unfold NDopsem.returnUpdateLocals.
+  rewrite J1. 
+  destruct (getCallerReturnID c); inv H1; eauto.
+    exists (updateAddAL GVs lc2' i0 gvs2).   
+    split; auto using instantiate_locals__updateAddAL.
+Qed.
+
+Lemma instantiate_locals__getIncomingValuesForBlockFromPHINodes : forall TD b
+    gl lc1 lc2 (Hlc : instantiate_locals lc1 lc2) ps re1,  
+  getIncomingValuesForBlockFromPHINodes TD ps b gl lc1 = Some re1 ->
+  exists re2,
+    NDopsem.getIncomingValuesForBlockFromPHINodes TD ps b gl lc2 = Some re2 /\
+    instantiate_locals re1 re2.
+Proof.
+  induction ps; simpl; intros.  
+    inv H. exists nil. simpl. auto.
+
+    destruct a.
+    destruct (getValueViaBlockFromValuels l0 b); tinv H.
+    remember (getOperandValue TD v lc1 gl) as R.
+    destruct R; tinv H.
+    symmetry in HeqR.  
+    eapply instantiate_locals__getOperandValue in HeqR; eauto.
+    destruct HeqR as [gvs2 [J1 J2]].
+    remember (getIncomingValuesForBlockFromPHINodes TD ps b gl lc1) as R1.
+    destruct R1; inv H.  
+    rewrite J1.
+    symmetry in HeqR1.
+    destruct (@IHps l1) as [re2 [J3 J4]]; auto.
+    rewrite J3. 
+    exists ((i0, gvs2) :: re2). simpl. auto.
+Qed.
+
+Lemma instantiate_locals__updateValuesForNewBlock : forall lc1 lc2 re1 re2,
+  instantiate_locals lc1 lc2 ->
+  instantiate_locals re1 re2 ->
+  instantiate_locals (updateValuesForNewBlock re1 lc1)
+     (NDopsem.updateValuesForNewBlock re2 lc2).
+Proof.
+  induction re1; destruct re2; simpl; intros; auto.
+    inv H0.
+    destruct a. inv H0.
+    destruct a. destruct p. destruct H0 as [eq [J1 J2]]; subst.
+    apply instantiate_locals__updateAddAL; auto.    
+Qed.
+
+Lemma instantiate_locals__switchToNewBasicBlock : forall TD lc1 lc2 gl lc1' b b',
+  instantiate_locals lc1 lc2 -> 
+  switchToNewBasicBlock TD b' b gl lc1 = Some lc1' ->
+  exists lc2', NDopsem.switchToNewBasicBlock TD b' b gl lc2 = Some lc2' /\
+    instantiate_locals lc1' lc2'. 
+Proof.
+  intros.
+  unfold switchToNewBasicBlock in H0.
+  unfold NDopsem.switchToNewBasicBlock.
+  remember (getIncomingValuesForBlockFromPHINodes TD (getPHINodesFromBlock b') b
+           gl lc1) as R.
+  destruct R; inv H0.
+  symmetry in HeqR.
+  eapply instantiate_locals__getIncomingValuesForBlockFromPHINodes in HeqR; eauto.
+  destruct HeqR as [re2 [J1 J2]].
+  rewrite J1.
+  exists (NDopsem.updateValuesForNewBlock re2 lc2).
+  split; auto using instantiate_locals__updateValuesForNewBlock.
+Qed.
+
+Lemma instantiate_gv__inhabited : forall gv gvs,
+  instantiate_gv gv gvs -> Inhabited _ gvs.
+Proof.
+  intros.
+  destruct gv; simpl in *.
+    apply Extensionality_Ensembles in H. subst.
+    apply singleton_inhabited.
+
+    destruct p.
+    destruct v; try solve [auto |
+      apply Extensionality_Ensembles in H; subst; apply singleton_inhabited].
+    destruct gv; try solve [auto |
+      apply Extensionality_Ensembles in H; subst; apply singleton_inhabited].
+Qed.
+
+Lemma mbop_is_total : forall TD bop0 sz0 x y, 
+  exists z, mbop TD bop0 sz0 x y = Some z.
+Proof.
+  intros.
+  unfold mbop.
+  destruct (GV2val TD x); eauto.
+  destruct v; eauto.
+  destruct (GV2val TD y); eauto.
+  destruct v; eauto.
+  destruct (eq_nat_dec (wz + 1) (Size.to_nat sz0)); eauto.
+  destruct bop0; eauto.
+Qed.
+
+Lemma instantiate_gv__mbop__helper : forall x xs y ys TD bop0 sz0
+  (H0 : instantiate_gv x xs)
+  (H1 : instantiate_gv y ys),
+   Inhabited GenericValue
+     (fun gv3 : GenericValue =>
+      exists gv1 : GenericValue,
+        exists gv2 : GenericValue,
+          exists gv3' : GenericValue,
+            gv1 @ xs /\
+            gv2 @ ys /\ mbop TD bop0 sz0 gv1 gv2 = ret gv3' /\ gv3 @ $ gv3' $).
+Proof.
+  intros.
+  apply instantiate_gv__inhabited in H0. inv H0.
+  apply instantiate_gv__inhabited in H1. inv H1.
+  destruct (@mbop_is_total TD bop0 sz0 x0 x1) as [z J].
+  assert (J1:=@gv2gvs__inhabited z). inv J1.
+  exists x2. unfold Ensembles.In. exists x0. exists x1. exists z.
+  split; auto. 
+Qed.
+
+Lemma instantiate_gv__mbop : forall TD bop0 sz0 x y z xs ys,
+  mbop TD bop0 sz0 x y = Some z ->
+  instantiate_gv x xs ->
+  instantiate_gv y ys ->
+  instantiate_gv z (lift_op2 (mbop TD bop0 sz0) xs ys).
+Proof.
+  intros. unfold lift_op2. 
+  destruct x; try solve [inv H; simpl; 
+      eapply instantiate_gv__mbop__helper; eauto].
+  destruct p.
+  destruct x; try solve [inv H; simpl; 
+      eapply instantiate_gv__mbop__helper; eauto].
+  destruct v; try solve [inv H; simpl; 
+      eapply instantiate_gv__mbop__helper; eauto].
+  destruct y; try solve [inv H; simpl; 
+      eapply instantiate_gv__mbop__helper; eauto].
+  destruct p.
+  destruct y; try solve [inv H; simpl; 
+      eapply instantiate_gv__mbop__helper; eauto].
+  destruct v; try solve [inv H; simpl; 
+      eapply instantiate_gv__mbop__helper; eauto].
+  apply Extensionality_Ensembles in H0. subst.
+  apply Extensionality_Ensembles in H1. subst.
+  assert (J1:=@gv2gvs__inhabited z). inv J1.
+
+  assert (exists v, exists c, z = (v,c)::nil) as EQ.
+    unfold mbop in H.
+    destruct (GV2val TD ((Vint wz i0, m) :: nil));
+      try solve [inv H; unfold gundef; simpl; eauto].
+    destruct v; try solve [inv H; unfold gundef; simpl; eauto].
+    destruct (eq_nat_dec (wz1 + 1) (Size.to_nat sz0));
+      try solve [inv H; unfold gundef; simpl; eauto].
+    destruct (GV2val TD ((Vint wz0 i1, m0) :: nil));
+      try solve [inv H; unfold gundef; simpl; eauto].
+    destruct v; try solve [inv H; unfold gundef; simpl; eauto].
+    unfold val2GV in *.
+    destruct bop0; try solve [inv H; unfold gundef; simpl; eauto].
+    
+  destruct EQ as [v [c EQ]]. subst.
+  simpl.   
+  destruct v.
+    exists x. exists ((Vint wz i0, m) :: nil). exists ((Vint wz0 i1, m0) :: nil).
+    exists ((Vundef, c) :: nil). 
+    repeat (split; try solve [auto | constructor]).
+
+    unfold Same_set, Included.
+    split; intros.
+      inv H1. unfold Ensembles.In. 
+      exists ((Vint wz i0, m) :: nil). exists ((Vint wz0 i1, m0) :: nil).
+      exists ((Vint wz1 i2, c) :: nil). 
+      repeat (split; try solve [auto | constructor]).
+
+      inv H1. unfold Ensembles.In. 
+      destruct H2 as [gv2 [gv3 [J1 [J2 [J3 J4]]]]].
+      inv J1. inv J2.
+      rewrite H in J3. inv J3. inv J4. constructor.
+
+    unfold Same_set, Included.
+    split; intros.
+      inv H1. unfold Ensembles.In. 
+      exists ((Vint wz i0, m) :: nil). exists ((Vint wz0 i1, m0) :: nil).
+      exists ((Vfloat f, c) :: nil). 
+      repeat (split; try solve [auto | constructor]).
+
+      inv H1. unfold Ensembles.In. 
+      destruct H2 as [gv2 [gv3 [J1 [J2 [J3 J4]]]]].
+      inv J1. inv J2.
+      rewrite H in J3. inv J3. inv J4. constructor.
+
+    unfold Same_set, Included.
+    split; intros.
+      inv H0. unfold Ensembles.In. 
+      exists ((Vint wz i0, m) :: nil). exists ((Vint wz0 i1, m0) :: nil).
+      exists ((Vptr b i2, c) :: nil). 
+      repeat (split; try solve [auto | constructor]).
+
+      inv H1. unfold Ensembles.In. 
+      destruct H2 as [gv2 [gv3 [J1 [J2 [J3 J4]]]]].
+      inv J1. inv J2.
+      rewrite H in J3. inv J3. inv J4. constructor.
+
+    unfold Same_set, Included.
+    split; intros.
+      inv H0. unfold Ensembles.In. 
+      exists ((Vint wz i0, m) :: nil). exists ((Vint wz0 i1, m0) :: nil).
+      exists ((Vinttoptr i2, c) :: nil). 
+      repeat (split; try solve [auto | constructor]).
+
+      inv H1. unfold Ensembles.In. 
+      destruct H2 as [gv2 [gv3 [J1 [J2 [J3 J4]]]]].
+      inv J1. inv J2.
+      rewrite H in J3. inv J3. inv J4. constructor.
+Qed.
+
+Lemma instantiate_locals__BOP : forall TD lc1 lc2 gl v1 v2 gv3 bop sz,
+  instantiate_locals lc1 lc2 -> 
+  BOP TD lc1 gl bop sz v1 v2 = Some gv3 ->
+  exists gvs3', NDopsem.BOP TD lc2 gl bop sz v1 v2 = Some gvs3' /\
+    instantiate_gv gv3 gvs3'.
+Proof.
+  intros.
+  apply BOP_inversion in H0.
+  destruct H0 as [gv1 [gv2 [J1 [J2 J3]]]].
+  eapply instantiate_locals__getOperandValue in J1; eauto.
+  destruct J1 as [gvs1 [H1 H2]].
+  eapply instantiate_locals__getOperandValue in J2; eauto.
+  destruct J2 as [gvs2 [H3 H4]].
+  unfold NDopsem.BOP.
+  rewrite H1. rewrite H3.
+  exists (lift_op2 (mbop TD bop0 sz0) gvs1 gvs2).
+  split; eauto using instantiate_gv__mbop.
+Qed.
+  
+Fixpoint instantiate_gvs (l1 : list GenericValue) (l2 : list GVs) :=
+match l1, l2 with
+| nil, nil => True
+| gv1::l1', gvs2::l2' => instantiate_gv gv1 gvs2 /\ instantiate_gvs l1' l2'
+| _, _ => False
+end.
+
+Lemma instantiate_locals__values2GVs : forall TD lc1 lc2 gl idxs vidxs,
+  instantiate_locals lc1 lc2 -> 
+  values2GVs TD idxs lc1 gl = Some vidxs ->
+  exists vidxss, NDopsem.values2GVs TD idxs lc2 gl = Some vidxss /\
+    instantiate_gvs vidxs vidxss.
+Proof.
+  induction idxs; simpl; intros.
+    inv H0. exists nil. simpl. auto.
+
+    remember (getOperandValue TD v lc1 gl) as R.
+    destruct R; tinv H0.
+    remember (values2GVs TD idxs lc1 gl) as R1.
+    destruct R1; inv H0.
+    symmetry in HeqR.
+    eapply instantiate_locals__getOperandValue in HeqR; eauto.
+    destruct HeqR as [gvs2 [H3 H4]].
+    destruct (@IHidxs l0) as [vidxss [J1 J2]]; auto.
+    rewrite H3. rewrite J1. exists (gvs2 :: vidxss). simpl. split; auto.
+Qed.
+
+Definition defined_gv (gv:GenericValue) : Prop :=
+match gv with
+| (v,_)::_ => v <> Vundef
+| _ => True
+end.
+
+Fixpoint defined_gvs (gvs:list GenericValue) : Prop :=
+match gvs with
+| gv::gvs' => defined_gv gv /\ defined_gvs gvs'
+| nil => True
+end.
+
+Lemma GV2ptr__defined_gv : forall TD sz ptr v, 
+  GV2ptr TD sz ptr = Some v -> defined_gv ptr.
+Proof.
+  intros.  
+  unfold GV2ptr in H.
+  destruct ptr; tinv H.
+  destruct p.
+  destruct v0; tinv H.
+  destruct ptr; inv H.
+  simpl. congruence.
+Qed.
+
+Lemma defined_gv__instantiate_gv : forall gv gvs,
+  defined_gv gv -> instantiate_gv gv gvs -> gv @ gvs.
+Proof.
+  destruct gv; simpl; intros.
+    apply Extensionality_Ensembles in H0. subst. 
+    constructor.
+
+    destruct p.
+    destruct v; try solve [
+      contradict H; auto |
+      apply Extensionality_Ensembles in H0; subst; constructor
+    ].
+Qed.      
+
+Lemma defined_gv__same_singleton : forall gv gvs,
+  defined_gv gv -> instantiate_gv gv gvs -> (Singleton GenericValue gv) = gvs.
+Proof.
+  destruct gv; simpl; intros.
+    apply Extensionality_Ensembles in H0. auto.
+
+    destruct p.
+    destruct v; try solve [
+      contradict H; auto |
+      apply Extensionality_Ensembles in H0; auto
+    ].
+Qed.      
+
+Lemma GV2int__defined_gv : forall TD sz gv v, 
+  GV2int TD sz gv = Some v -> defined_gv gv.
+Proof.
+  intros.  
+  unfold GV2int in H.
+  destruct gv; tinv H.
+  destruct p.
+  destruct v0; tinv H.
+  destruct gv; inv H.
+  simpl. congruence.
+Qed.
+
+Lemma GVs2Nats__defined_gvs : forall TD vidxs idxs, 
+  GVs2Nats TD vidxs = Some idxs -> defined_gvs vidxs.
+Proof.
+  induction vidxs; simpl; intros; auto.
+  
+  remember (GV2int TD Size.ThirtyTwo a) as R.
+  destruct R; tinv H.
+  remember (GVs2Nats TD vidxs) as R1.
+  destruct R1; inv H.
+  symmetry in HeqR.
+  apply GV2int__defined_gv in HeqR.
+  split; eauto.
+Qed.
+
+Lemma defined_gvs__instantiate_gvs : forall gv gvs,
+  defined_gvs gv -> instantiate_gvs gv gvs -> gv @@ gvs.
+Proof.
+  induction gv; intros.
+    destruct gvs; inv H0.
+    simpl. auto.
+
+    simpl in H0.
+    destruct gvs; inv H0.
+    simpl. simpl in H. destruct H.
+    apply defined_gv__instantiate_gv in H1; auto.
+Qed.
+
+Fixpoint singletons (l1 : list GenericValue) (l2 : list GVs) :=
+match l1, l2 with
+| nil, nil => True
+| gv1::l1', gvs2::l2' => (Singleton GenericValue gv1) = gvs2 /\ 
+                            singletons l1' l2'
+| _, _ => False
+end.
+
+Lemma defined_gvs__same_singleton : forall gv gvs,
+  defined_gvs gv -> instantiate_gvs gv gvs -> singletons gv gvs.
+Proof.
+  induction gv; intros.
+    destruct gvs; inv H0.
+    simpl. auto.
+
+    simpl in H0.
+    destruct gvs; inv H0.
+    simpl. simpl in H. destruct H.
+    apply defined_gv__same_singleton in H1; auto.
+Qed.
+
+Lemma singletons_spec : forall gv1 gvs gv2,
+  singletons gv1 gvs -> gv2 @@ gvs -> gv1 = gv2.
+Proof.
+  induction gv1; simpl; intros.
+    destruct gvs; inv H.
+    destruct gv2; inv H0; auto.
+
+    destruct gvs; inv H.
+    destruct gv2; simpl in H0; inv H0.
+    inv H. eapply IHgv1 in H2; eauto.
+    subst. auto.
+Qed.
+
+Lemma GEP_is_total : forall TD t mp vidxs inbounds0,
+  exists mp', LLVMgv.GEP TD t mp vidxs inbounds0 = ret mp'.
+Proof.
+  intros. unfold LLVMgv.GEP. 
+  destruct (GV2ptr TD (getPointerSize TD) mp); eauto.
+  destruct (GVs2Nats TD vidxs); eauto.
+  destruct (mgep TD t v l0); eauto.
+Qed.
+
+Lemma instantiate_gvs__inhabited : forall gv gvs,
+  instantiate_gvs gv gvs -> exists gv1, gv1 @@ gvs.
+Proof.
+  induction gv; simpl in *; intros.
+    destruct gvs; inv H.
+    exists nil. simpl. auto.
+
+    destruct gvs; inv H.
+    destruct (@IHgv gvs) as [gv1 J]; auto.
+    apply instantiate_gv__inhabited in H0.
+    inv H0.
+    exists (x::gv1). simpl. auto.
+Qed.    
+
+Lemma instantiate_locals__GEP_helper : forall vidxs vidxss mp1 mps2 TD t
+  inbounds (Hinst1 : instantiate_gvs vidxs vidxss)
+  (Hinst2 : instantiate_gv mp1 mps2),
+   Inhabited GenericValue
+     (fun gv : GenericValue =>
+      exists ma : GenericValue,
+        exists vidxs0 : list GenericValue, exists gv',
+          ma @ mps2 /\
+          vidxs0 @@ vidxss /\ GEP TD t ma vidxs0 inbounds = ret gv' /\
+          gv @ $ gv' $ ).
+Proof.
+  intros.
+  apply instantiate_gvs__inhabited in Hinst1. destruct Hinst1 as [gv1 Hinst1].
+  apply instantiate_gv__inhabited in Hinst2. inv Hinst2.
+  destruct (@GEP_is_total TD t x gv1 inbounds0) as [gv2 J].
+  assert (J1:=@gv2gvs__inhabited gv2). inv J1.
+  exists x0. unfold Ensembles.In. exists x. exists gv1. exists gv2.
+  split; auto. 
+Qed.  
+
+Lemma instantiate_locals__GEP : forall TD t mp1 mp1' vidxs vidxss inbounds mps2,
+  instantiate_gvs vidxs vidxss ->
+  instantiate_gv mp1 mps2 ->
+  GEP TD t mp1 vidxs inbounds = Some mp1' ->
+  exists mps2', NDopsem.GEP TD t mps2 vidxss inbounds = Some mps2' /\ 
+    instantiate_gv mp1' mps2'.
+Proof.
+  intros TD t mp1 mp1' vidxs vidxss inbounds mps2 Hinst1 Hinst2 Hgep.
+  unfold NDopsem.GEP.
+  exists (fun gv : GenericValue =>
+        exists ma : GenericValue,
+          exists vidxs0 : list GenericValue,
+            exists gv' : GenericValue,
+              ma @ mps2 /\
+              vidxs0 @@ vidxss /\
+              GEP TD t ma vidxs0 inbounds = ret gv' /\ gv @ $ gv' $).
+  split; auto. 
+  unfold GEP in Hgep.
+  remember (GV2ptr TD (getPointerSize TD) mp1) as R.
+  destruct R; try solve [inv Hgep; simpl; 
+      eapply instantiate_locals__GEP_helper; eauto].
+  remember (GVs2Nats TD vidxs) as R1.
+  destruct R1; try solve [inv Hgep; simpl; 
+      eapply instantiate_locals__GEP_helper; eauto].
+  remember (mgep TD t v l0) as R2.
+  destruct R2; try solve [inv Hgep; simpl; 
+      eapply instantiate_locals__GEP_helper; eauto].
+  inv Hgep. 
+  unfold mgep in HeqR2.
+  destruct v; tinv HeqR2.
+  destruct l0; tinv HeqR2.
+  remember (mgetoffset TD (typ_array 0%nat t) (z :: l0)) as R3.
+  destruct R3 as [[o ?]|]; inv HeqR2.
+  unfold ptr2GV, val2GV. simpl.
+  symmetry in HeqR.
+  assert (J:=HeqR).
+  apply GV2ptr__defined_gv in J. 
+  apply defined_gv__same_singleton in Hinst2; auto. subst.
+  symmetry in HeqR1.
+  assert (J1:=HeqR1).
+  apply GVs2Nats__defined_gvs in J1. 
+  assert (J9:=Hinst1).
+  apply defined_gvs__instantiate_gvs in J9; auto. 
+  apply defined_gvs__same_singleton in Hinst1; auto. 
+  unfold Same_set, Included.
+  split; intros.
+    inv H. unfold Ensembles.In.
+    exists mp1.
+    exists vidxs. 
+    exists ((Vptr b (Int.add 31 i0 o), AST.Mint (getPointerSize TD - 1)) :: nil).
+    repeat (split; auto).
+    unfold GEP. rewrite HeqR. rewrite HeqR1. unfold mgep.
+    rewrite <- HeqR3. unfold ptr2GV, val2GV. auto.
+
+    inv H. destruct H0 as [A [B [J1' [J2 [J3 J4]]]]].
+    eapply singletons_spec in Hinst1; eauto. subst.
+    inv J1'. unfold GEP in J3.
+    rewrite HeqR in J3. rewrite HeqR1 in J3. unfold mgep in J3.
+    rewrite <- HeqR3 in J3. inv J3. inv J4.
+    unfold ptr2GV, val2GV. 
+    unfold Ensembles.In. constructor.
+Qed.
+
+Lemma mcast_is_total : forall TD cop0 t1 t2 x, 
+  exists z, mcast TD cop0 t1 t2 x = Some z.
+Proof.
+  intros.
+  unfold mcast, mbitcast.
+  destruct cop0; destruct t1; destruct t2; eauto.
+Qed.
+
+Lemma instantiate_gv__mcast__helper : forall x xs TD op t1 t2
+  (H0 : instantiate_gv x xs),
+   Inhabited GenericValue
+     (fun gv2 : GenericValue =>
+      exists gv1 : GenericValue,
+        exists gv2' : GenericValue,
+            gv1 @ xs /\ mcast TD op t1 t2 gv1 = ret gv2' /\ gv2 @ $ gv2' $).
+Proof.
+  intros.
+  apply instantiate_gv__inhabited in H0. inv H0.
+  destruct (@mcast_is_total TD op t1 t2 x0) as [z J].
+  assert (J1:=@gv2gvs__inhabited z). inv J1.
+  exists x1. unfold Ensembles.In. exists x0. exists z.
+  split; auto. 
+Qed.
+
+Lemma instantiate_gv__mcast__helper2 : forall z xs
+  (H0 : instantiate_gv z xs),
+   instantiate_gv z
+     (fun gv2 : GenericValue =>
+      exists gv1 : GenericValue,
+        exists gv2' : GenericValue,
+          gv1 @ xs /\ ret gv1 = ret gv2' /\ gv2 @ $ gv2' $).
+Proof.
+  intros.
+  destruct z.
+    apply Extensionality_Ensembles in H0. subst. 
+    simpl. 
+    unfold Same_set, Included.
+    split; intros.
+      inv H. unfold Ensembles.In. exists nil. exists nil. simpl.
+      split. constructor. split; auto. constructor. 
+
+      inv H. destruct H0 as [A [J1 [J2 J3]]]. inv J1. inv J2. inv J3.
+      unfold Ensembles.In. constructor.
+
+    destruct p. 
+    destruct v; simpl in *.
+      destruct z.
+        inv H0.  
+        assert (J:=@gv2gvs__inhabited x). inv J.
+        exists x0. unfold Ensembles.In. exists x. exists x.
+        split; auto.
+             
+        apply Extensionality_Ensembles in H0. subst. 
+        unfold Same_set, Included.
+        split; intros.
+          inv H. unfold Ensembles.In. exists ((Vundef, m) :: p :: z). 
+          exists ((Vundef, m) :: p :: z). simpl.
+          split. constructor. split; auto. constructor. 
+
+          inv H. destruct H0 as [A [J1 [J2 J3]]]. inv J1. inv J2. inv J3.
+          constructor.
+   
+     apply Extensionality_Ensembles in H0. subst. 
+     unfold Same_set, Included.
+     split; intros.
+        inv H. unfold Ensembles.In. exists ((Vint wz i0, m) :: z). 
+        exists ((Vint wz i0, m) :: z). simpl.
+        split. constructor. split; auto. constructor. 
+
+        inv H. destruct H0 as [A [J1 [J2 J3]]]. inv J1. inv J2. inv J3.
+        constructor.
+
+     apply Extensionality_Ensembles in H0. subst. 
+     unfold Same_set, Included.
+     split; intros.
+        inv H. unfold Ensembles.In. exists ((Vfloat f, m) :: z). 
+        exists ((Vfloat f, m) :: z). simpl.
+        split. constructor. split; auto. constructor. 
+
+        inv H. destruct H0 as [A [J1 [J2 J3]]]. inv J1. inv J2. inv J3.
+        constructor.
+
+     apply Extensionality_Ensembles in H0. subst. 
+     unfold Same_set, Included.
+     split; intros.
+        inv H. unfold Ensembles.In. exists ((Vptr b i0, m) :: z). 
+        exists ((Vptr b i0, m) :: z). simpl.
+        split. constructor. split; auto. constructor. 
+
+        inv H. destruct H0 as [A [J1 [J2 J3]]]. inv J1. inv J2. inv J3.
+        constructor.
+
+     apply Extensionality_Ensembles in H0. subst. 
+     unfold Same_set, Included.
+     split; intros.
+        inv H. unfold Ensembles.In. exists ((Vinttoptr i0, m) :: z). 
+        exists ((Vinttoptr i0, m) :: z). simpl.
+        split. constructor. split; auto. constructor. 
+
+        inv H. destruct H0 as [A [J1 [J2 J3]]]. inv J1. inv J2. inv J3.
+        constructor.
+Qed.
+
+Lemma instantiate_gv__mcast : forall TD cop0 t1 t2 x z xs,
+  mcast TD cop0 t1 t2 x = Some z ->
+  instantiate_gv x xs ->
+  instantiate_gv z (lift_op1 (mcast TD cop0 t1 t2) xs).
+Proof.
+  intros. unfold lift_op1. 
+  unfold mcast, mbitcast in H.
+Opaque mcast. 
+  destruct cop0; try solve [inv H; simpl; 
+      eapply instantiate_gv__mcast__helper; eauto];
+    destruct t1; destruct t2; try solve [    
+      inv H; destruct f; 
+        try solve [simpl; eapply instantiate_gv__mcast__helper; eauto] |
+      inv H; destruct f0; 
+        try solve [simpl; eapply instantiate_gv__mcast__helper; eauto] |
+      inv H; try solve [simpl; eapply instantiate_gv__mcast__helper; eauto]
+    ].
+Transparent mcast. 
+    inv H; unfold mcast, mbitcast; apply instantiate_gv__mcast__helper2; auto.
+    inv H; unfold mcast, mbitcast; apply instantiate_gv__mcast__helper2; auto.
+    inv H; unfold mcast, mbitcast; apply instantiate_gv__mcast__helper2; auto.
+    inv H; unfold mcast, mbitcast; apply instantiate_gv__mcast__helper2; auto.
+    inv H; unfold mcast, mbitcast; apply instantiate_gv__mcast__helper2; auto.
+    inv H; unfold mcast, mbitcast; apply instantiate_gv__mcast__helper2; auto.
+    inv H; unfold mcast, mbitcast; apply instantiate_gv__mcast__helper2; auto.
+    inv H; unfold mcast, mbitcast; apply instantiate_gv__mcast__helper2; auto.
+    inv H; unfold mcast, mbitcast; apply instantiate_gv__mcast__helper2; auto.
+    inv H; unfold mcast, mbitcast; apply instantiate_gv__mcast__helper2; auto.
+Qed.    
+
+Lemma instantiate_locals__CAST : forall TD lc1 lc2 gl t1 v1 t2 gv2 castop0,
+  instantiate_locals lc1 lc2 -> 
+  CAST TD lc1 gl castop0 t1 v1 t2 = Some gv2 ->
+  exists gvs2', NDopsem.CAST TD lc2 gl castop0 t1 v1 t2 = Some gvs2' 
+    /\ instantiate_gv gv2 gvs2'.
+Proof.
+  intros.
+  apply CAST_inversion in H0.
+  destruct H0 as [gv1 [J1 J2]].
+  eapply instantiate_locals__getOperandValue in J1; eauto.
+  destruct J1 as [gvs1 [H1 H2]].
+  unfold NDopsem.CAST.
+  rewrite H1.
+  exists (lift_op1 (mcast TD castop0 t1 t2) gvs1).
+  split; eauto using instantiate_gv__mcast.
+Qed.
+
+Lemma lookupFdefViaGV_inversion : forall TD Ps gl lc fs fv f,
+  lookupFdefViaGV TD Ps gl lc fs fv = Some f ->
+  exists fptr, exists fn,
+    getOperandValue TD fv lc gl = Some fptr /\
+    lookupFdefViaGVFromFunTable fs fptr = Some fn /\
+    lookupFdefViaIDFromProducts Ps fn = Some f.
+Proof.
+  intros.
+  unfold lookupFdefViaGV in H.
+  destruct (getOperandValue TD fv lc gl); tinv H.
+  simpl in H. exists g.
+  destruct (lookupFdefViaGVFromFunTable fs g); tinv H.
+  simpl in H. exists i0. eauto.
+Qed.  
+
+Lemma lookupFdefViaPtr_inversion : forall Ps fs fptr f,
+  lookupFdefViaPtr Ps fs fptr = Some f ->
+  exists fn,
+    lookupFdefViaGVFromFunTable fs fptr = Some fn /\
+    lookupFdefViaIDFromProducts Ps fn = Some f.
+Proof.
+  intros.
+  unfold lookupFdefViaPtr in H.
+  destruct (lookupFdefViaGVFromFunTable fs fptr); tinv H.
+  simpl in H. exists i0. eauto.
+Qed.  
+
+Lemma instantiate_locals__params2GVs : forall TD lc1 lc2 gl 
+  (Hlc:instantiate_locals lc1 lc2) lp gvs1,
+  params2GVs TD lp lc1 gl = Some gvs1 ->
+  exists gvss2, NDopsem.params2GVs TD lp lc2 gl = Some gvss2 /\
+    instantiate_gvs gvs1 gvss2.
+Proof.
+  induction lp; simpl; intros.
+    inv H. exists nil. simpl. auto.
+
+    destruct a.
+    remember (getOperandValue TD v lc1 gl) as R1.
+    destruct R1; tinv H.
+    remember (params2GVs TD lp lc1 gl) as R2.
+    destruct R2; tinv H.
+    inv H.
+    symmetry in HeqR1.
+    eapply instantiate_locals__getOperandValue in HeqR1; eauto.
+    destruct HeqR1 as [gvs2 [H3 H4]].
+    destruct (@IHlp l0) as [gvsss2 [J1 J2]]; auto.
+    rewrite H3. rewrite J1. exists (gvs2 :: gvsss2). simpl. split; auto.
+Qed.
+
+Lemma instantiate_locals__initializeFrameValues : forall lc1 lc2
+  (H2: instantiate_locals lc1 lc2) la gvs1 gvs2 (H1 : instantiate_gvs gvs1 gvs2),
+  instantiate_locals (_initializeFrameValues la gvs1 lc1)
+                     (NDopsem._initializeFrameValues la gvs2 lc2).
+Proof.
+  induction la; simpl; intros; auto.
+    destruct a. destruct p.
+    destruct gvs1; simpl.
+      destruct gvs2; inv H1.
+      apply instantiate_locals__updateAddAL; auto using instantiate_gv__gv2gvs. 
+        apply IHla. simpl. auto.
+
+      simpl in H1.
+      destruct gvs2; inv H1.
+      apply instantiate_locals__updateAddAL; auto.
+Qed.           
+
+Lemma instantiate_locals__initLocals : forall gvs1 gvss2 
+  (H : instantiate_gvs gvs1 gvss2) la,
+  instantiate_locals (initLocals la gvs1) (NDopsem.initLocals la gvss2).
+Proof.
+  unfold initLocals, NDopsem.initLocals.
+  intros.
+  apply instantiate_locals__initializeFrameValues; simpl; auto.
+Qed.
+
+Lemma defined_gv_dec : forall gv, defined_gv gv \/ ~ defined_gv gv.
+Proof.
+  destruct gv; simpl; auto.
+    destruct p; simpl; auto.
+    destruct v; simpl; try solve [left; congruence].
+      right. intro J. contradict J; auto.
+Qed.      
+
+Lemma defined_gvs_dec : forall gvs, defined_gvs gvs \/ ~ defined_gvs gvs.
+Proof.
+  induction gvs; simpl; auto.
+    destruct IHgvs as [IHgvs | IHgvs].
+      destruct (@defined_gv_dec a) as [J | J]; auto.
+        right. intros [J1 J2]. congruence.
+      right. intros [J1 J2]. congruence.
+Qed.
+
+Lemma malloc__defined_gv : forall TD M tsz gn align0 M' mb,
+  malloc TD M tsz gn align0 = Some (M', mb) ->
+  defined_gv gn.
+Proof.
+  intros.
+  apply malloc_inv in H.
+  destruct H as [n [J1 [J2 J3]]].
+  unfold GV2int in J1.
+  destruct gn; tinv J1.
+  destruct p.
+  destruct v; tinv J1. simpl. congruence.
+Qed. 
+  
+Lemma free__defined_gv : forall TD M ptr M',
+  free TD M ptr = Some M' ->
+  defined_gv ptr.
+Proof.
+  intros.
+  apply free_inv in H.
+  destruct H as [blk [ofs [hi [lo [J1 [J2 [J3 J4]]]]]]].
+  unfold GV2ptr in J1.
+  destruct ptr; tinv J1.
+  destruct p.
+  destruct v; tinv J1. simpl. congruence.
+Qed. 
+
+Lemma mload_inv : forall Mem2 t align0 TD gvp2 
+  (gv2 : GenericValue)
+  (H21 : mload TD Mem2 gvp2 t align0 = ret gv2),
+  exists b, exists ofs, exists m, gvp2 = (Vptr b ofs,m)::nil.
+Proof.
+  intros.
+  unfold mload in H21.
+  remember (GV2ptr TD (getPointerSize TD) gvp2) as R.
+  destruct R; try solve [inversion H21].
+  destruct v; try solve [inversion H21].
+  unfold GV2ptr in HeqR.
+  destruct gvp2; try solve [inversion HeqR].
+  destruct p.
+  destruct v; try solve [inversion HeqR].
+  destruct gvp2; inv HeqR.
+  exists b0. exists i1. 
+  unfold ptr2GV, val2GV. eauto.
+Qed.
+
+Lemma mload__defined_gv : forall TD M ptr t a gv,
+  mload TD M ptr t a = Some gv ->
+  defined_gv ptr.
+Proof.
+  intros.
+  apply mload_inv in H.
+  destruct H as [blk [ofs [m J1]]].
+  inv J1. simpl. congruence.
+Qed. 
+
+Lemma mstore__defined_gv : forall TD M ptr t a gv M',
+  mstore TD M ptr t gv a = Some M' ->
+  defined_gv ptr.
+Proof.
+  intros.
+  apply store_inv in H.
+  destruct H as [blk [ofs [c [v0 [J1 [J2 [J3 J4]]]]]]].
+  unfold GV2ptr in J1. 
+  destruct ptr; tinv J1.
+  destruct p.
+  destruct v; tinv J1.
+  destruct ptr; inv J1.
+  simpl. congruence.
+Qed. 
+
+Definition undef_state St : Prop :=
+  match St with 
+  | {| CurTargetData := TD;
+       ECS := {| CurCmds := nil;
+                 Terminator := insn_br _ Cond _ _;
+                 Locals := lc |} :: _;
+       Globals := gl |} =>
+     match getOperandValue TD Cond lc gl with
+     | ret c => ~ defined_gv c 
+     | _ => False
+     end
+  | {| CurTargetData := TD;
+       ECS := {| CurCmds := insn_store _ _ v _ _::_;
+                 Locals := lc |} :: _;
+       Globals := gl |} =>
+     match getOperandValue TD v lc gl with
+     | ret gv => ~ defined_gv gv 
+     | _ => False
+     end
+  | {| CurTargetData := TD;
+       ECS := {| CurCmds := insn_call _ _ _ _ fv _::_;
+                 Locals := lc |} :: _;
+       Globals := gl |} =>
+     match getOperandValue TD fv lc gl with
+     | ret gv => ~ defined_gv gv 
+     | _ => False
+     end
+  | _ => False
+  end.
+
+Lemma instantiate_dsInsn : forall st1 st2 st1' tr,
+  instantiate_State st1 st2 ->
+  LLVMopsem.dsInsn st1 st1' tr ->
+  (exists st2', sInsn st2 st2' tr /\ instantiate_State st1' st2') \/
+  undef_state st1.
+Proof.
+  intros st1 st2 st1' tr Hsim Hop.  
+  (dsInsn_cases (induction Hop) Case).
+Case "dsReturn". simpl_nd_llvmds. 
+  eapply instantiate_locals__returnUpdateLocals in H1; eauto.
+  destruct H1 as [lc2'' [H1 H2]].
+  left. exists (NDopsem.mkState S' TD' Ps' 
+    ((NDopsem.mkEC f2' b2' cs' tmn2' lc2'' als2')::ECs') gl' fs' Mem').
+  split; eauto.
+    repeat (split; auto).
+Case "dsReturnVoid". simpl_nd_llvmds. 
+  left. exists (NDopsem.mkState S' TD' Ps' 
+    ((NDopsem.mkEC f2' b2' cs' tmn2' lc2' als2')::ECs') gl' fs' Mem').
+  split; eauto.
+    repeat (split; auto).
+Case "dsBranch". simpl_nd_llvmds. 
+  simpl. rewrite H.
+  destruct (@defined_gv_dec c) as [Hdet | Hndet]; auto.
+  left.
+  eapply instantiate_locals__switchToNewBasicBlock in H1; eauto.
+  eapply instantiate_locals__getOperandValue in H; eauto.
+  destruct H as [gvs2 [J1 J2]].
+  destruct H1 as [lc2' [J3 J4]].
+  apply defined_gv__instantiate_gv in J2; auto.   
+  exists (NDopsem.mkState S' TD' Ps' 
+    ((NDopsem.mkEC f1' (block_intro l' ps' cs' tmn') cs' tmn' lc2' als1')
+      ::ECs') gl' fs' M').
+  split; eauto.
+    repeat (split; auto).
+Case "dsBranch_uncond". simpl_nd_llvmds. 
+  eapply instantiate_locals__switchToNewBasicBlock in H0; eauto.
+  destruct H0 as [lc2' [J1 J2]]. left.
+  exists (NDopsem.mkState S' TD' Ps' 
+    ((NDopsem.mkEC f1' (block_intro l' ps' cs' tmn') cs' tmn' lc2' als1')
+      ::ECs') gl' fs' M').
+  split; eauto.
+    repeat (split; auto).
+Case "dsBop". simpl_nd_llvmds. 
+  eapply instantiate_locals__BOP in H; eauto.
+  destruct H as [gvs3' [J1 J2]]. left.
+  exists (NDopsem.mkState S' TD' Ps' 
+    ((NDopsem.mkEC f1' b1' cs tmn1' (updateAddAL _ lc1' id0 gvs3') als1')
+      ::ECs') gl' fs' M').
+  split; eauto.
+    repeat (split; auto using instantiate_locals__updateAddAL).
+Case "dsFBop". admit.
+Case "dsExtractValue". admit.
+Case "dsInsertValue". admit.
+Case "dsMalloc". simpl_nd_llvmds. 
+  assert (J:=H1).
+  apply malloc__defined_gv in J.
+  left.
+  eapply instantiate_locals__getOperandValue in H0; eauto.
+  destruct H0 as [gns [J1 J2]].
+  apply defined_gv__instantiate_gv in J2; auto.   
+  exists (NDopsem.mkState S' TD' Ps' 
+    ((NDopsem.mkEC f1' b1' cs tmn1' 
+      (updateAddAL _ lc1' id0 ($ (blk2GV TD' mb) $)) 
+    als1')::ECs') gl' fs' Mem').
+  split; eauto.
+    repeat (split; auto using instantiate_locals__updateAddAL, 
+                              instantiate_gv__gv2gvs).
+Case "dsFree". simpl_nd_llvmds. 
+  assert (J:=H0).
+  apply free__defined_gv in J.
+  left.
+  eapply instantiate_locals__getOperandValue in H; eauto.
+  destruct H as [gvs [J1 J2]].
+  apply defined_gv__instantiate_gv in J2; auto.   
+  exists (NDopsem.mkState S' TD' Ps' 
+    ((NDopsem.mkEC f1' b1' cs tmn1' lc1'
+    als1')::ECs') gl' fs' Mem').
+  split; eauto. 
+    repeat (split; auto).
+Case "dsAlloca". simpl_nd_llvmds. 
+  assert (J:=H1).
+  apply malloc__defined_gv in J.
+  left.
+  eapply instantiate_locals__getOperandValue in H0; eauto.
+  destruct H0 as [gns [J1 J2]].
+  apply defined_gv__instantiate_gv in J2; auto.   
+  exists (NDopsem.mkState S' TD' Ps' 
+    ((NDopsem.mkEC f1' b1' cs tmn1' 
+      (updateAddAL _ lc1' id0 ($ (blk2GV TD' mb) $)) 
+    (mb::als1'))::ECs') gl' fs' Mem').
+  split; eauto.
+    repeat (split; auto using instantiate_locals__updateAddAL, 
+                              instantiate_gv__gv2gvs).
+Case "dsLoad". simpl_nd_llvmds.
+  assert (J:=H0).
+  apply mload__defined_gv in J.
+  left.
+  eapply instantiate_locals__getOperandValue in H; eauto.
+  destruct H as [gvs2 [J1 J2]].
+  apply defined_gv__instantiate_gv in J2; auto.   
+  exists (NDopsem.mkState S' TD' Ps' 
+    ((NDopsem.mkEC f1' b1' cs tmn1' (updateAddAL _ lc1' id0 ($ gv $))
+    als1')::ECs') gl' fs' M').
+  split; eauto. 
+    repeat (split; auto using instantiate_locals__updateAddAL, 
+                              instantiate_gv__gv2gvs).
+Case "dsStore". simpl_nd_llvmds.
+  assert (J:=H1).
+  apply mstore__defined_gv in J.
+  simpl. rewrite H.
+  destruct (@defined_gv_dec gv1) as [Hdet | Hndet]; auto.
+  left.
+  eapply instantiate_locals__getOperandValue in H; eauto.
+  destruct H as [gvs2 [J1 J2]].
+  apply defined_gv__instantiate_gv in J2; auto.   
+  eapply instantiate_locals__getOperandValue in H0; eauto.
+  destruct H0 as [mps2 [J3 J4]].
+  apply defined_gv__instantiate_gv in J4; auto.   
+  exists (NDopsem.mkState S' TD' Ps' 
+    ((NDopsem.mkEC f1' b1' cs tmn1' lc1' als1')::ECs') gl' fs' Mem').
+  split; eauto. 
+    repeat (split; auto).
+Case "dsGEP". simpl_nd_llvmds. 
+  eapply instantiate_locals__getOperandValue in H; eauto.
+  destruct H as [mps [J1 J2]].
+  eapply instantiate_locals__values2GVs in H0; eauto.
+  destruct H0 as [vidxss [J3 J4]].
+  eapply instantiate_locals__GEP in H1; eauto.
+  destruct H1 as [mps2' [J5 J6]]. left.
+  exists (NDopsem.mkState S' TD' Ps' 
+    ((NDopsem.mkEC f1' b1' cs tmn1' (updateAddAL _ lc1' id0 mps2') als1')
+      ::ECs') gl' fs' M').
+  split; eauto.
+    repeat (split; auto using instantiate_locals__updateAddAL).
+Case "dsTrunc". admit.
+Case "dsExt". admit.
+Case "dsCast". simpl_nd_llvmds. left.
+  eapply instantiate_locals__CAST in H; eauto.
+  destruct H as [gvs2' [J1 J2]].
+  exists (NDopsem.mkState S' TD' Ps' 
+    ((NDopsem.mkEC f1' b1' cs tmn1' (updateAddAL _ lc1' id0 gvs2') als1')
+      ::ECs') gl' fs' M').
+  split; eauto.
+    repeat (split; auto using instantiate_locals__updateAddAL).
+Case "dsIcmp". admit.
+Case "dsFcmp". admit.
+Case "dsSelect". admit.
+Case "dsCall". simpl_nd_llvmds. 
+  apply lookupFdefViaGV_inversion in H.
+  destruct H as [fptr [fn [J1 [J2 J3]]]].
+  simpl. rewrite J1.
+  destruct (@defined_gv_dec fptr) as [Hdet | Hndet]; auto.
+  left.
+  eapply instantiate_locals__getOperandValue in J1; eauto.
+  destruct J1 as [gvs2 [J11 J12]].
+  apply defined_gv__instantiate_gv in J12; auto.   
+  eapply instantiate_locals__params2GVs in H1; eauto.
+  destruct H1 as [gvss2 [H11 H12]].
+  exists (NDopsem.mkState S' TD' Ps' 
+    ((NDopsem.mkEC (fdef_intro (fheader_intro fa rt fid la va) lb) 
+                       (block_intro l' ps' cs' tmn') cs' tmn' 
+                       (NDopsem.initLocals la gvss2) 
+                       nil)::
+     (NDopsem.mkEC f1' b1' (insn_call rid noret0 ca ft fv lp :: cs) tmn1' 
+      lc1' als1') ::ECs') gl' fs' M').
+  split.
+    eapply sCall; eauto.
+      unfold lookupFdefViaPtr. 
+      rewrite J2. simpl. rewrite J3. auto.
+    repeat (split; auto using instantiate_locals__initLocals).
+Case "dsExCall". admit.
+Qed.
+
+(*****************************)
+(*
+*** Local Variables: ***
+*** coq-prog-name: "coqtop" ***
+*** coq-prog-args: ("-emacs-U" "-I" "~/SVN/sol/vol/src/ssa/monads" "-I" "~/SVN/sol/vol/src/ssa/ott" "-I" "~/SVN/sol/vol/src/ssa/compcert" "-I" "~/SVN/sol/theory/metatheory_8.3") ***
+*** End: ***
+ *)
